src/kernel/standard_kernel.cpp
@@ -5,7 +5,7 @@ Released under Apache 2.0 license as described in the file LICENSE.
 Author: Leonardo de Moura
 */
 #include "kernel/inductive/inductive.h"
-#include "kernel/quotient/quotient.h"
+#include "kernel/computation/computation.h"
 
 namespace lean {
 using inductive::inductive_normalizer_extension;
@@ -15,6 +15,6 @@ environment mk_environment(unsigned trust_lvl) {
     return environment(trust_lvl,
                        /* builtin support for inductive */
                        compose(std::unique_ptr<normalizer_extension>(new inductive_normalizer_extension()),
-                               std::unique_ptr<normalizer_extension>(new quotient_normalizer_extension())));
+                               std::unique_ptr<normalizer_extension>(new computation_normalizer_extension())));
 }
 }
