src/library/noncomputable.h
@@ -13,6 +13,8 @@ bool is_marked_noncomputable(environment const & env, name const & n);
 bool is_noncomputable(environment const & env, name const & n);
 /** \brief Mark \c n as noncomputable */
 environment mark_noncomputable(environment const & env, name const & n);
+/** \brief Mark \c n as computable. */
+environment bless_computable(environment const & env, name const & n);
 /** \brief In standard mode, check if definitions that are not propositions can compute */
 bool check_computable(environment const & env, name const & n);
 optional<name> get_noncomputable_reason(environment const & env, name const & n);
