tests/lean/quot_bug.lean
@@ -1,9 +1,11 @@
-open quot
+open quotient
 variables {A : Type} {B : A → Type}
 
 variable f : Π a : A, B a
 
-#reduce λ x, quot.lift_on ⟦f⟧ (λf : (Πx : A, B x), f) _ x
+variable [setoid (Π a, B a)]
 
-example (x : A) : quot.lift_on ⟦f⟧ (λf : (Πx : A, B x), f) sorry x = f x :=
+#reduce λ x, quotient.lift_on ⟦f⟧ (λf : (Πx : A, B x), f) _ x
+
+example (x : A) : quotient.lift_on ⟦f⟧ (λf : (Πx : A, B x), f) sorry x = f x :=
 rfl
